\subsection{}

We denote the subspace~$X × \{ y_0 \} ∪ \{ x_0 \} × Y$ of~$X × Y$ by~$Z$.

The two continuous maps
\[
	f_X
	\colon
	X \to Z \,,
	\quad
	x \mapsto (x, y_0)
\]
and
\[
	f_Y
	\colon
	Y \to Z \,,
	\quad
	y \mapsto (x_0, y)
\]
assemble into a single continuous map
\[
	f' \colon X + Y \to Z \,.
\]
This map satisfies~$f'(x_0) = (x_0, y_0) = f'(y_0)$, and therefore factors through a continuous map
\[
	f \colon X ∨ Y \to Z \,,
\]
The map~$f$ is already bijective.
It remains to show that it is open.

Let~$U$ be an open subset of~$X ∨ Y$.
It’s preimage in~$X + Y$ is a saturated open subset.
It is thus of the form~$V_X + V_Y$ for open subsets~$V_X$ and~$V_Y$ of~$X$ and~$Y$ respectively, such that~$x_0 ∈ V_X$ if and only if~$y_0 ∈ V_Y$.
We have
\[
	f(U)
	=
	f'(V_X + V_Y)
	=
	f_X(V_X) ∪ f_Y(V_Y)
	=
	V_X × \{ y_0 \} ∪ \{ x_0 \} × V_Y \,.
\]
We distinguish between two cases:
\begin{casedistinction}

	\item
		Suppose that~$x_0 ∈ V_X$ and~$y_0 ∈ V_Y$.
		The set~$V_X × V_Y$ is open in~$X × Y$, whence the set
		\begin{align*}
			(V_X × V_Y) ∩ Z
			&=
			(V_X × V_Y) ∩ (X × \{ y_0 \} ∪ \{ x_0 \} × Y)
			\\
			&=
			((V_X × V_Y) ∩ (X × \{ y_0 \})) ∪ ((V_X × V_Y) ∩ (\{ x_0 \} × Y))
			\\
			&=
			V_X × \{ y_0 \} ∪ \{ x_0 \} × V_Y
			\\
			&=
			f(U)
		\end{align*}
		is open in~$Z$.

	\item
		Suppose that~$x_0 ∉ V_X$ and~$y_0 ∉ V_Y$.
		The set~$V_X × Y ∪ X × V_Y$ is open in~$X × Y$, whence the set
		\begin{align*}
			{}&
			(V_X × Y ∪ X × V_Y) ∩ Z
			\\
			={}&
			(V_X × Y ∪ X × V_Y) ∩ (X × \{ y_0 \} ∪ \{ x_0 \} × Y)
			\\
			={}&
			  ((V_X × Y) ∩ (X × \{ y_0 \}))
			∪ ((V_X × Y) ∩ (\{ x_0 \} × Y))
			\\
			{}&
			∪ ((X × V_Y) ∩ (X × \{ y_0 \}))
			∪ ((X × V_Y) ∩ (\{ x_0 \} × Y))
			\\
			={}&
			V_X × \{ y_0 \}
			∪ ∅ × Y
			∪ X × ∅
			∪ \{ x_0 \} × V_Y
			\\
			={}&
			V_X × \{ y_0 \} ∪ \{ x_0 \} × V_Y
			\\
			={}&
			f(U)
		\end{align*}
		is open in~$Z$.

\end{casedistinction}
We find in both cases that~$f(U)$ is open in~$Z$.
